acyclic_sigma -> acyclic

theories/lang.v
@@ -280,7 +280,7 @@ Proof.
   by move=> /andP[yk ts]; rewrite in_fnd yk ts.
 Qed.
 
-Definition acyclic_sigma (s: Sigma) := [disjoint domf s & codom_vars s].
+Definition acyclic (s: Sigma) := [disjoint domf s & codom_vars s].
 
 Lemma add_some T (x z: T): Some x = Some z -> x = z. by move=> []. Qed.
 
@@ -332,11 +332,11 @@ Proof.
 Qed.
 
 Lemma acyclic_sigma_set s k v:
-  acyclic_sigma s.[k <- v] = 
-    [&& acyclic_sigma s.[~k], (k \notin vars_tm v), (k \notin codom_vars s.[~k]) &
+  acyclic s.[k <- v] = 
+    [&& acyclic s.[~k], (k \notin vars_tm v), (k \notin codom_vars s.[~k]) &
       fdisjoint (domf s) (vars_tm v)].
 Proof.
-  rewrite /acyclic_sigma dom_setf fdisjointUX fdisjoint1X !codom_vars_set.
+  rewrite /acyclic dom_setf fdisjointUX fdisjoint1X !codom_vars_set.
   rewrite !fdisjointXU; rewrite !inE; case: (boolP (_ \in _)); rewrite ?(andbF,andbT)// => ks.
   rewrite domf_rem orFb; case: (boolP (_ \in _)); rewrite ?(andbF,andbT)// => ksf.
   rewrite andTb.
@@ -350,7 +350,7 @@ Proof.
   by rewrite xsk in ks.
 Qed.
 
-Lemma acyclic_sigma_rem s k: acyclic_sigma s -> acyclic_sigma s.[\ k].
+Lemma acyclic_sigma_rem s k: acyclic s -> acyclic s.[\ k].
 Proof.
   move=> H; apply/fdisjointWr/fdisjointWl/H.
     by rewrite codom_vars_sub.
@@ -360,8 +360,8 @@ Qed.
 Lemma empty_rem k: empty.[~k] = empty.
 Proof. by apply/fmapP => p;rewrite fnd_rem1 not_fnd//if_same. Qed.
 
-Lemma acyclic_sigma0: acyclic_sigma empty.
-Proof. by rewrite/acyclic_sigma fdisjoint0X. Qed.
+Lemma acyclic_sigma0: acyclic empty.
+Proof. by rewrite/acyclic fdisjoint0X. Qed.
 
 Lemma codom0: codom empty = [::].
 Proof. by rewrite /empty codomE/= enum_fset0. Qed.
@@ -369,25 +369,25 @@ Proof. by rewrite /empty codomE/= enum_fset0. Qed.
 Lemma codom_vars0: codom_vars empty = fset0.
 Proof. by rewrite/codom_vars codom0. Qed.
 
-Goal ~ (acyclic_sigma [fmap].[IV 0 <- Tm_V (IV 0)]).
+Goal ~ (acyclic [fmap].[IV 0 <- Tm_V (IV 0)]).
 Proof. by rewrite acyclic_sigma_set empty_rem acyclic_sigma0 codom_vars0 fdisjoint0X/= !inE. Qed.
 
-Goal ~ (acyclic_sigma [fmap].[IV 0 <- Tm_V (IV 1)].[IV 1 <- Tm_V (IV 0)]).
+Goal ~ (acyclic [fmap].[IV 0 <- Tm_V (IV 1)].[IV 1 <- Tm_V (IV 0)]).
 Proof. by rewrite acyclic_sigma_set !inE remf1_id ?inE// codom_vars_set !inE/= eqxx orbT/= andbF. Qed.
 
-Goal ~ (acyclic_sigma [fmap].[IV 0 <- Tm_V (IV 1)].[IV 1 <- Tm_V (IV 0)].[IV 2 <- Tm_P (IP 1)]).
+Goal ~ (acyclic [fmap].[IV 0 <- Tm_V (IV 1)].[IV 1 <- Tm_V (IV 0)].[IV 2 <- Tm_P (IP 1)]).
 Proof.
   rewrite acyclic_sigma_set remf1_id?inE// acyclic_sigma_set inE.
   by rewrite remf1_id?inE//= fdisjointX0 andbT codom_vars_set !inE/= eqxx orbT/= andbF.
 Qed.
 
-Goal (acyclic_sigma [fmap].[IV 0 <- Tm_V (IV 1)]).
+Goal (acyclic [fmap].[IV 0 <- Tm_V (IV 1)]).
 Proof.
   by rewrite acyclic_sigma_set empty_rem acyclic_sigma0 codom_vars0 !inE fdisjoint0X.
 Qed.
 
 Definition acyclic_ren (m: {fmap V -> V}) := 
-  (* acyclic_sigma [fmap s => Tm_V m.[valP s]]. *)
+  (* acyclic [fmap s => Tm_V m.[valP s]]. *)
   [disjoint domf m & codomf m].
 
 Lemma acyclic_ren0: acyclic_ren ctx.empty.
@@ -481,7 +481,7 @@ Lemma deref_V s v: deref s (Tm_V v) = odflt (Tm_V v) (s.[?v]).
 Proof. by []. Qed.
 
 Lemma deref2' s e t:
-  acyclic_sigma (s+e) -> deref (s+e) (deref e t) = deref (s+e) t.
+  acyclic (s+e) -> deref (s+e) (deref e t) = deref (s+e) t.
 Proof.
   move=> A; elim: t => //[v|/=f->a->//].
   rewrite !deref_V fnd_cat.
@@ -497,7 +497,7 @@ Lemma catf2 (K:choiceType) V (s: {fmap K -> V}): s + s = s.
 Proof. by apply/fmapP => x; rewrite fnd_cat if_same. Qed.
 
 Lemma deref2 s t:
-  (acyclic_sigma s) -> deref s (deref s t) = deref s t.
+  (acyclic s) -> deref s (deref s t) = deref s t.
 Proof. by have:= @deref2' s s t; rewrite catf2. Qed.
 
 Lemma vars_tm_deref_sub s t:
@@ -541,7 +541,7 @@ Proof.
 Qed.
 
 Lemma acyclic_deref_disjoint s t:
-  acyclic_sigma s -> [disjoint domf s & vars_tm (deref s t)].
+  acyclic s -> [disjoint domf s & vars_tm (deref s t)].
 Proof.
   move=> A; elim: t => //=; only 1: by rewrite fdisjointX0.
     move=> v; case: fndP => //=vs.
@@ -674,7 +674,7 @@ Variable u : Unif.
 Definition bc : program -> fvS -> Tm -> Sigma -> fvS * seq (Sigma * seq Atom) :=
 (*ENDSNIP: bc_type*)
   fun pr fv (query:Tm) s =>
-  if ~~ acyclic_sigma s then (fv, [::])
+  if ~~ acyclic s then (fv, [::])
   else
   let query := deref s query in
   let: (fv, rules) := fresh_rules (vars_sigma s `|` vars_tm query `|` fv) (pr.(rules)) in
@@ -749,7 +749,7 @@ Proof. by rewrite/ground/=; apply:contraFF erefl => /eqP/fsetP /(_ v); rewrite !
 Lemma ground_app f a: ground (Tm_App f a) = ground f && ground a.
 Proof. by rewrite /ground/= fsetU_eq0. Qed.
 
-Lemma acyclic_sigma_set_D k t: ground t -> acyclic_sigma empty.[k <- t].
+Lemma acyclic_sigma_set_D k t: ground t -> acyclic empty.[k <- t].
 Proof.
   rewrite acyclic_sigma_set empty_rem fdisjoint0X acyclic_sigma0 codom_vars0.
   by rewrite /ground => /eqP->//.
